Some refactoring of relational examples, made cache example more interesting

examples/relational/cache.fst
@@ -11,31 +11,82 @@ open Comp
 open Heap
 open List
 
-val fib : nat -> Tot nat
-let rec fib x = if x <= 1 then 1 else  fib (x-1) + fib (x-2)
+(* Functional Sepcification of Factorials *)
+val fac : nat -> Tot nat
+let rec fac x = if x = 0 then 1 else  fac (x-1) * x
 
-type fib_cache = list (nat * nat)
-assume val cache : ref fib_cache
+(* A tail-recursive imperative implementation *)
+val imp_fac : x:ref nat -> a:ref nat 
+  -> ST nat (requires (fun h -> a <> x))
+            (ensures  (fun h r h' -> a <> x 
+                                  /\ r = (fac (sel h x) * (sel h a))
+                                  /\ sel h' x = 0 
+                                  /\ sel h' a = r
+                                  /\ modifies (a ^+^ x) h h'))
+let rec imp_fac x a = 
+  if !x = 0 then 
+    !a 
+  else 
+  ( a := !a * !x;
+    x := !x -1;
+    imp_fac x a)
 
-type fib_cache_correct (c:fib_cache) = (forall x. is_Some (assoc x c) ==> (Some.v (assoc x c) = fib x))
+(* A wrapper for the recursive function, ensuring that the heap will not be
+   modified *)
+val imp_fac_wrap : x:ref nat -> a:ref nat -> y:nat 
+  -> ST nat (requires  (fun h -> a <> x))
+            (ensures   (fun h r h' -> r = fac y 
+                                       /\ modifies Set.empty h h'))
+let imp_fac_wrap x a y =
+  let tmp1 = !x in 
+  let tmp2 = !a in
+  x := y;
+  a := 1;
+  let res = imp_fac x a in 
+  x := tmp1;
+  a := tmp2;
+  res
 
-(*
-val fib_cached : x:nat -> ST nat (requires (fun h -> fib_cache_correct (sel h cache)))
-                               (ensures  (fun _ r h ->  fib_cache_correct (sel h cache)
-                                                        /\ r = fib x))
-*)
-let (fib_cached x):nat =
+type fac_cache = list (nat * nat)
+assume val cache : ref fac_cache
+
+(* An invariant on the correctness of the cache *)
+type fac_cache_correct (c:fac_cache) = (forall x. is_Some (assoc x c) ==> (Some.v (assoc x c) = fac x))
+
+(* A cached version of the factorial computation *)
+val fac_cached : x:nat -> ST nat (requires (fun h -> fac_cache_correct (sel h cache)))
+                                 (ensures  (fun h r h' ->  fac_cache_correct (sel h' cache)
+                                                        /\ modifies (only cache) h h'
+                                                        /\ r = fac x))
+let fac_cached x =
   let c = !cache in
   let l = assoc x c in
   if is_Some l then
     Some.v l
   else(
-    let v = fib x in
+    let v = fac x in
     cache := (x,v) :: c;
-    fib x)
+    fac x)
 
-val correct : eq nat
+(* Can we maybe proof this? (modifies is defined based on equality..) *)
+(* Maybe it is also better to define an own predicate for this, because we are
+   somehow "abusing" modifies for a different purpose *)
+assume val heap_modifies_refl : h0:heap -> h1:heap -> mods:Set.set Heap.aref
+  -> Lemma (requires (modifies mods h0 h1))
+           (ensures  (modifies mods h1 h0))
+(* let heap_modifies_refl h0 h1 mods = () *)
+
+(* Proof that the functions compute the same values and that cache is the only
+   memory cell that can be modified *)
+val correct : x:ref nat -> a:ref nat -> y:eq nat
   -> ST2 (eq nat)
-         (requires (fun h -> fib_cache_correct (sel (R.r h) cache)))
-         (ensures (fun _ _ h -> fib_cache_correct (sel (R.r h) cache)))
-let correct x = compose2 (fun x -> fib x) (fun x -> fib_cached x) x
+         (requires (fun h -> fac_cache_correct (sel (R.r h) cache)
+                          /\ x <> a 
+                          /\ modifies (only cache) (R.l h) (R.r h)))
+         (ensures (fun h _ h' -> fac_cache_correct (sel (R.r h') cache)
+                              /\ modifies (only cache) (R.l h') (R.r h')))
+let correct x a y =   let h = compose2_self ST.get (twice ()) in 
+                      let res = compose2 (fun y -> imp_fac_wrap x a y) (fun x -> fac_cached x) y in
+                      let h' = compose2_self ST.get (twice ()) in 
+                      heap_modifies_refl (R.l h) (R.l h') (Set.empty);
+                      res
